checkpoint a different plan
all the abstract state stays the same (indexed by nat, etc) but the
executable operations must supply the string versions of the same
nats we used to pass before.  seems like this should be less tedious,
but need to flesh this out a bit more..

src/Mail/MailServerAPI.v
@@ -8,7 +8,6 @@ Definition string: Type := abstract_string.
 Parameter tmp_string : string.
 Parameter mail_string : string.
 Parameter nouser_string : string.
-Parameter empty_string : string.
 Parameter bench_msg : string.
 Parameter tmp_mail_ne : tmp_string <> mail_string.
 Parameter abstract_string_length : string -> nat.
@@ -18,8 +17,21 @@ Instance string_Ordering : Ordering string.
 Admitted.
 
 Parameter nat_to_string : nat -> string.
-Axiom nat_to_string_eq : forall a b,
+Parameter string_to_nat : string -> nat.
+Axiom nat_to_string_to_nat : forall a,
+  string_to_nat (nat_to_string a) = a.
+
+Definition natpair_to_stringpair '(a, b) := (nat_to_string a, nat_to_string b).
+
+Theorem nat_to_string_eq : forall a b,
   nat_to_string a = nat_to_string b -> a = b.
+Proof.
+  intros.
+  rewrite <- nat_to_string_to_nat.
+  rewrite <- H.
+  rewrite nat_to_string_to_nat.
+  reflexivity.
+Qed.
 
 Theorem nat_to_string_ne : forall a b,
   a <> b -> nat_to_string a <> nat_to_string b.
@@ -89,7 +101,7 @@ Module MailServerHOp := HOps MailServerOp UserIdx.
 
 Module MailServerState <: State.
 
-  Definition dir_contents := FMap.t (string*string) string.
+  Definition dir_contents := FMap.t (nat*nat) string.
 
   Definition State := dir_contents.
   Definition initP (s : State) := True.
@@ -124,11 +136,11 @@ Module MailServerAPI <: Layer MailServerOp MailServerState.
     FMap.is_permutation_kv r mbox ->
     xstep Pickup tid
       mbox
-      r
+      (map (fun '(fn, msg) => (natpair_to_stringpair fn, msg)) r)
       mbox
       nil
   | StepDelete : forall mbox tid id,
-    xstep (Delete id) tid
+    xstep (Delete (natpair_to_stringpair id)) tid
       mbox
       tt
       (FMap.remove id mbox)
