src/Mail/MailFSAPI.v
@@ -40,7 +40,7 @@ Module MailFSAPI <: Layer MailFSOp MailboxTmpAbsState.
     xstep (CreateWriteTmp data) tid
       (mk_state tmp mbox lock)
       true
-      (mk_state (FMap.add (tid, empty_string) data tmp) mbox lock)
+      (mk_state (FMap.add (nat_to_string tid, nat_to_string 0) data tmp) mbox lock)
       nil
   | StepCreateWriteTmpErr1 : forall tmp mbox tid data lock,
     xstep (CreateWriteTmp data) tid
@@ -52,21 +52,21 @@ Module MailFSAPI <: Layer MailFSOp MailboxTmpAbsState.
     xstep (CreateWriteTmp data) tid
       (mk_state tmp mbox lock)
       false
-      (mk_state (FMap.add (tid, 0) data' tmp) mbox lock)
+      (mk_state (FMap.add (nat_to_string tid, nat_to_string 0) data' tmp) mbox lock)
       nil
   | StepUnlinkTmp : forall tmp mbox tid lock,
     xstep (UnlinkTmp) tid
       (mk_state tmp mbox lock)
       tt
-      (mk_state (FMap.remove (tid, 0) tmp) mbox lock)
+      (mk_state (FMap.remove (nat_to_string tid, nat_to_string 0) tmp) mbox lock)
       nil
   | StepLinkMailOK : forall tmp mbox tid mailfn data lock,
-    FMap.MapsTo (tid, 0) data tmp ->
-    ~ FMap.In (tid, mailfn) mbox ->
-    xstep (LinkMail mailfn) tid
+    FMap.MapsTo (nat_to_string tid, nat_to_string 0) data tmp ->
+    ~ FMap.In (nat_to_string tid, nat_to_string mailfn) mbox ->
+    xstep (LinkMail (nat_to_string mailfn)) tid
       (mk_state tmp mbox lock)
       true
-      (mk_state tmp (FMap.add (tid, mailfn) data mbox) lock)
+      (mk_state tmp (FMap.add (nat_to_string tid, nat_to_string mailfn) data mbox) lock)
       nil
   | StepLinkMailErr : forall tmp mbox tid mailfn lock,
     xstep (LinkMail mailfn) tid
